theories/weakestpre.v
@@ -6,31 +6,78 @@ From iris.algebra Require Import gmap excl auth.
 From iris.program_logic Require weakestpre.
 From iris.program_logic Require Import ownp.
 
-From self Require Export vprop view lang.
+From self Require Export dprop view lang.
 From self.lang Require Import primitive_laws syntax.
 
 Section wp.
   Context `{!nvmG Σ}.
 
-  Implicit Types (Φ : val → vProp Σ) (e : expr).
-  (* (P Q : vProp Σ) (E : coPset) *)
+  Implicit Types (Φ : val → dProp Σ) (e : expr).
+  (* (P Q : dProp Σ) (E : coPset) *)
 
-  (* Our weakest precondition is a [vProp]. We construct it using [MonPred]
+  (* Global Instance fst_lat_mono : Proper ((⊑) ==> (⊑)) (@fst A B).
+  Proof. move => [??][??][-> _]//. Qed.
+
+  Global Instance snd_lat_mono : Proper ((⊑) ==> (⊑)) (@snd A B).
+  Proof. move => [??][??][_ ->]//. Qed. *)
+
+  Global Instance store_view_mono : Proper ((⊑) ==> (⊑)) store_view.
+  Proof.
+    intros [[??]?] [[??]?].
+    rewrite /sqsubseteq /subseteq_thread_view /subseteq_view.
+    rewrite !pair_included.
+    intros [[le _] _].
+    done.
+  Qed.
+
+  Global Instance persist_view_mono : Proper ((⊑) ==> (⊑)) persist_view.
+  Proof.
+    intros [[??]?] [[??]?].
+    rewrite /sqsubseteq /subseteq_thread_view /subseteq_view.
+    rewrite !pair_included.
+    intros [[_ le] _].
+    done.
+  Qed.
+
+  Global Instance wb_buffer_view_mono : Proper ((⊑) ==> (⊑)) wb_buffer_view.
+  Proof.
+    intros [[??]?] [[??]?].
+    rewrite /sqsubseteq /subseteq_thread_view /subseteq_view.
+    rewrite !pair_included.
+    intros [_ le].
+    done.
+  Qed.
+
+  (* Program Definition test' P : dProp Σ :=
+    MonPred (λ V,
+      ∀ TV, ⌜V ⊑ TV⌝ -∗ P)%I _.
+  Next Obligation. solve_proper. Qed. *)
+
+  (* Program Definition test P : dProp Σ :=
+    MonPred (λ V,
+      ∀ TV, ⌜(store_view V) ⊑ (store_view TV)⌝ -∗ P)%I _.
+  Next Obligation. solve_proper. Qed. *)
+
+  (* Our weakest precondition is a [dProp]. We construct it using [MonPred]
   which wraps the function along with a proof that it is monotone. *)
-  Program Definition wp_def s E e Φ : vProp Σ :=
+  Program Definition wp_def s E e Φ : dProp Σ :=
     MonPred (λ V,
       ∀ TV,
-        ⌜V ⊑ TV.(tv_store_view)⌝ -∗
-        valid (TV.(tv_store_view)) -∗
+        (* ⌜TV ⊑ V⌝ -∗ *)
+        ⌜(store_view V) ⊑ (store_view TV)⌝ -∗
+        ⌜(persist_view V) ⊑ (persist_view TV)⌝ -∗
+        ⌜(wb_buffer_view V) ⊑ (wb_buffer_view TV)⌝ -∗
+        valid (store_view TV) -∗
         WP (ThreadState e TV) @ s; E {{ λ res,
-          let '(ThreadVal v TV') := res return _ in (Φ v TV'.(tv_store_view))
+          let '(ThreadVal v TV') := res return _ in
+            valid (store_view TV') ∗ (Φ v TV')
         }})%I _.
   Next Obligation. solve_proper. Qed.
 
   (* This is sealing follows the same ritual as the [wp] in Iris. *)
   Definition wp_aux : seal (@wp_def). by eexists. Qed.
 
-  Global Instance expr_wp : Wp expr_lang (vProp Σ) stuckness := wp_aux.(unseal).
+  Global Instance expr_wp : Wp expr_lang (dProp Σ) stuckness := wp_aux.(unseal).
 
   Lemma wp_eq : wp = wp_def.
   Proof. rewrite -wp_aux.(seal_eq). done. Qed.
@@ -43,16 +90,38 @@ Section wp.
     Proper (pointwise_relation val (≡) ==> (≡)) (wp s E e).
   Proof. rewrite wp_eq. constructor=>V. solve_proper. Qed.
 
-  Lemma wp_value_fupd s E Φ e v : IntoVal e v → WP e @ s; E {{ Φ }} ⊣⊢ |={E}=> Φ v.
+  Lemma wp_value_fupd' s E Φ v : WP of_val v @ s; E {{ Φ }} ⊣⊢ |={E}=> Φ v.
   Proof.
-    intros <-.
-  Abort.
+    rewrite wp_eq. rewrite /wp_def.
+    iStartProof (iProp _). simpl. iIntros (TV'). iSplit.
+    - iIntros "hi". admit.
+    - iIntros "HΦ **".
+      iApply (weakestpre.wp_value_fupd' _ _ _ (ThreadVal v TV)).
+      iFrame.
+  Admitted.
+      (* epose proof (weakestpre.wp_value_fupd' s E _ (ThreadVal v TV)).
+      simpl in *.
+      rewrite H2.
+      iApply weakestpre.wp_value_fupd'. *)
+      (* rewrite -(weakestpre.wp_value_fupd' _ _ (Φ v)). *)
+      (* iDestruct (weakestpre.wp_value_fupd' with "HΦ") as "HI". *)
+      (* rewrite -wp_value_fupd'.
+      iApply (wp_value' _ _ _ (ThreadVal v _)). iFrame.
+    rewrite wp_value_fupd'.
+  Admitted. *)
+
+  (* Definition prop : dProp Σ := ⎡⌜1 =2⌝⎤%I. *)
+
+  (* Definition prop' : dProp Σ := (⎡⌜1 =2⌝⎤ -∗ True)%Ig *)
+
+  Lemma wp_value_fupd s E Φ e v : IntoVal e v → WP e @ s; E {{ Φ }} ⊣⊢ |={E}=> Φ v.
+  Proof. intros <-. by apply wp_value_fupd'. Qed.
 
   (* If the expression is a value then showing the postcondition for the value
   suffices. *)
   Lemma wp_value s E Φ v : Φ v ⊢ WP (of_val v) @ s; E {{ Φ }}.
   Proof.
-    iStartProof (iProp _). simpl. rewrite wp_eq /wp_def. iIntros "% HΦ %% ?".
+    iStartProof (iProp _). simpl. rewrite wp_eq /wp_def. iIntros "% HΦ %% ? ??".
     iApply (wp_value' _ _ _ (ThreadVal v _)). iFrame.
   Qed.
 
