theories/dprop.v
@@ -1,0 +1,28 @@
+(* In this file we define [dProp], the type of propositions in the high-level
+logic. *)
+
+From iris.bi Require Export monpred big_op.
+From iris.proofmode Require Import tactics monpred modality_instances.
+From iris.base_logic.lib Require Import fancy_updates.
+
+From self Require Import view memory.
+
+Instance subseteq_thread_view : SqSubsetEq thread_view :=
+  λ TV TV', TV ≼ TV'.
+
+(* We define a canonical [biIndex] structure for [thread_view]. All fields except for
+[bi_index_type] can be infered by Coq. *)
+Canonical Structure thread_view_bi_index : biIndex :=
+  {| bi_index_type := thread_view; |}.
+
+(* Uncomment this to see the fields that Coq infer. *)
+Print thread_view_bi_index.
+
+Instance view_bi_index_bot (TV : thread_view) : BiIndexBottom (ε : thread_view).
+Proof. apply: ucmra_unit_least. Qed.
+
+(* Types of view predicates. *)
+Definition dProp Σ := monPred thread_view_bi_index (uPredI (iResUR Σ)). (* FIXME: use iPropI here. *)
+Definition dPropO Σ := monPredO thread_view_bi_index (uPredI (iResUR Σ)).
+Definition dPropI Σ := monPredI thread_view_bi_index (uPredI (iResUR Σ)).
+
